MirrorCharge!/src/MirrorCharge/ModularFunc/SubstType.v
@@ -3,6 +3,8 @@ Require Import ExtLib.Data.PreFun.
 
 Require Import MirrorCore.TypesI.
 
+Require Import MirrorCharge.ModularFunc.BaseType.
+
 Require Import Charge.Open.Subst.
 Require Import Charge.Open.Stack.
 
@@ -13,7 +15,6 @@ Set Strict Implicit.
 Set Maximal Implicit Insertion.
 
 Class SubstType (typ : Type) := {
-  tyVar : typ;
   tyVal : typ;
   tySubst : typ
 }.
@@ -21,9 +22,10 @@ Class SubstType (typ : Type) := {
 Section SubstTypeD.
 	Context {typ : Type} {HT : SubstType typ} {HR : RType typ}.
 	Context {VN : ValNull (typD tyVal)}.
+	Context {BT : BaseType typ}.
 
 	Class SubstTypeD := {
-	  stSubst : typD tySubst = @subst (typD tyVar) (typD tyVal)
+	  stSubst : typD tySubst = @subst (typD tyString) (typD tyVal)
 	}.
 	
 End SubstTypeD.
