MirrorCharge!/src/MirrorCharge/RTac/RTac.v
@@ -1,0 +1,9 @@
+Require Export MirrorCharge.RTac.Apply.
+Require Export MirrorCharge.RTac.Cancellation.
+Require Export MirrorCharge.RTac.EApply.
+Require Export MirrorCharge.RTac.Instantiate.
+Require Export MirrorCharge.RTac.Intro.
+Require Export MirrorCharge.RTac.Minify.
+Require Export MirrorCharge.RTac.PullConjunct.
+Require Export MirrorCharge.RTac.ReifyLemma.
+Require Export MirrorCharge.RTac.Subst.
